LwRust/Paper.lean
@@ -2,6 +2,7 @@ import LwRust.Paper.Syntax
 import LwRust.Paper.Runtime
 import LwRust.Paper.InductiveSemantics
 import LwRust.Paper.Typing
+import LwRust.Paper.BorrowChecker
 import LwRust.Paper.Soundness
 import LwRust.Paper.Soundness.Index
 import LwRust.Paper.Examples
